src/proof/controllers/replicaset.v
@@ -19,15 +19,137 @@ Definition current_state_matches rs pods : Prop :=
   | None => False
   end.
 
-Lemma wp_syncReplicaSet γ l (gv: schema.GroupVersion.t) namespace name uid rs pods :
+Lemma wp_manageReplicas γ l (gv: schema.GroupVersion.t) sl rs_l ptrs pods rs n dq1 dq2 :
   {{{ is_pkg_init code.controllers.replicaset.replicaset ∗
       "#Hisk" ∷ is_kubernetes γ l ∗
       "#Hglobal_l" ∷ (global_addr common.State) ↦□ l ∗
       "#Hglobal_gv" ∷ (global_addr v1.SchemeGroupVersion) ↦□ gv ∗
-      "Hown_rs_meta_frag" ∷ own_meta_frag γ (ReplicaSetV.key rs) uid 1 rs.(ReplicaSetV.ObjectMeta') ∗
+      "Hsl" ∷ sl ↦* ptrs ∗
+      "Hdeepown_l_pods" ∷ ([∗ list] ptr;pod ∈ ptrs;pods, PodV.deepown_l ptr pod dq1) ∗
+      "Hdeepown_l_rs" ∷ ReplicaSetV.deepown_l rs_l rs dq2 ∗
+      "Hown_pod_meta_frags" ∷ ([∗ list] pod ∈ pods,
+        own_meta_frag γ (PodV.key pod) pod.(PodV.ObjectMeta').(ObjectMetaV.UID') 1 pod.(PodV.ObjectMeta')) ∗
+      "Hown_children_frag" ∷ own_children_frag γ (ReplicaSetV.key rs)
+        rs.(ReplicaSetV.ObjectMeta').(ObjectMetaV.UID') 1 (list_to_set (PodV.key <$> pods)) ∗
+      "%Hrs_valid" ∷ ⌜ ReplicaSetV.valid rs ⌝ ∗
+      "%Hrs_name_short" ∷ ⌜ length rs.(ReplicaSetV.ObjectMeta').(ObjectMetaV.Name') < 58 ⌝ ∗
+      "%Hpods_active" ∷ ⌜ Forall is_pod_alive pods ⌝ ∗
+      "%Hreplicas_eq" ∷ ⌜ rs.(ReplicaSetV.Spec').(ReplicaSetSpecV.Replicas') = Some n ⌝
+  }}}
+    @! replicaset.manageReplicas #sl #rs_l
+  {{{ pods', RET #interface.nil;
+      ⌜ length pods' = sint.nat n ⌝ ∗
+      ⌜ Forall is_pod_alive pods' ⌝ ∗
+      sl ↦* ptrs ∗
+      ([∗ list] ptr;pod ∈ ptrs;pods, PodV.deepown_l ptr pod dq1) ∗
+      ReplicaSetV.deepown_l rs_l rs dq2 ∗
+      ([∗ list] pod ∈ pods',
+        own_meta_frag γ (PodV.key pod) pod.(PodV.ObjectMeta').(ObjectMetaV.UID') 1 pod.(PodV.ObjectMeta')) ∗
+      own_children_frag γ (ReplicaSetV.key rs)
+        rs.(ReplicaSetV.ObjectMeta').(ObjectMetaV.UID') 1 (list_to_set (PodV.key <$> pods'))
+  }}}.
+Proof.
+  wp_start as "H". iNamed "H". wp_auto.
+  iPoseProof (ReplicaSetV.deepown_l_split with "Hdeepown_l_rs") as
+    "(Hdeepown_t_l_rs & Hdeepown_m_l_rs & Hdeepown_s_l_rs & Hdeepown_st_l_rs)".
+  iDestruct "Hdeepown_s_l_rs" as "(%rs_spec_c & Hrs_spec_l & Hdeepown_rs_spec)".
+  iNamedPrefix "Hdeepown_rs_spec" "Hrs_".
+  iAssert ((rs_spec_c.(v1.ReplicaSetSpec.Replicas') ↦{dq2} n)%I) with "[Hrs_Hdeepown_replicas_some]"
+    as "Hrs_Hdeepown_replicas".
+  { rewrite Hreplicas_eq. iDestruct "Hrs_Hdeepown_replicas_some" as "(%replicas & Hreplicas & ->)". done. }
+  wp_auto.
+  iDestruct (own_slice_len with "Hsl") as %(Hsl_len1 & Hsl_len2).
+  iDestruct (own_slice_wf with "Hsl") as %Hsl_cap.
+  iDestruct (big_sepL2_length with "Hdeepown_l_pods") as %Hlen.
+  assert (0 ≤ sint.Z n) as Hn.
+  { destruct Hrs_valid as (_ & Hrs_spec_valid & _).
+    pose proof (ReplicaSetSpecV.valid_replicas _ Hrs_spec_valid) as (i & Hi_eq & Hi).
+    rewrite Hi_eq in Hreplicas_eq. congruence. }
+  assert ((sint.Z (word.sub (slice.len_f sl) (W64 (sint.Z n)))) = (sint.Z (slice.len_f sl)) - (sint.Z n)) as -> by word.
+  assert ((sint.Z (W64 0)) = 0) as -> by word.
+  wp_if_destruct.
+  - set I := (∃ (i: w64) (pods': list PodV.t),
+      "Hi_ptr" ∷ i_ptr ↦ i ∗
+      "Hown_pod_meta_frags" ∷ ([∗ list] pod ∈ pods',
+        own_meta_frag γ (PodV.key pod) pod.(PodV.ObjectMeta').(ObjectMetaV.UID') 1 pod.(PodV.ObjectMeta')) ∗
+      "Hown_children_frag" ∷ own_children_frag γ (ReplicaSetV.key rs)
+        rs.(ReplicaSetV.ObjectMeta').(ObjectMetaV.UID') 1 (list_to_set (PodV.key <$> pods')) ∗
+      "%Hpods_active'" ∷ ⌜ Forall is_pod_alive pods' ⌝ ∗
+      "%Hlength_eq'" ∷ ⌜ length pods' = Z.to_nat ((sint.Z (slice.len_f sl)) + sint.Z i) ⌝ ∗
+      "%Hi" ∷ ⌜ 0 ≤ sint.Z i ≤ sint.Z (word.mul (word.sub (slice.len_f sl) (W64 (sint.Z n))) (W64 (-1))) ⌝
+    )%I.
+    iAssert (I) with "[i Hown_pod_meta_frags Hown_children_frag]" as "Hloop_inv".
+    { iExists (W64 0), pods. iFrame. iPureIntro. split_and!; [done|word|word|word]. }
+    wp_for "Hloop_inv". wp_if_destruct.
+    + wp_apply wp_globals_get. wp_apply schema.wp_GroupVersion__WithKind.
+      { (* TODO: why? *) iAssert (is_pkg_init code.k8s_io.api.apps.v1.v1) as "H". all: iPkgInit. }
+      iIntros (gvk) "%Hgvk". wp_auto.
+      destruct Hgvk as (Hgvk_g & Hgvk_v & Hgvk_k).
+      wp_apply (v1.wp_NewControllerRef_ReplicaSet with "[$Hdeepown_m_l_rs]"); [done|].
+      iIntros (controller_ref_l controller_ref) "(Hdeepown_l_controller_ref & %Hcontroller_ref_valid &
+        Hdeepown_m_l_rs)". wp_auto. rewrite Hgvk_k in Hcontroller_ref_valid.
+      iDestruct (struct_fields_split with "Hrs_spec_l") as "H". iNamedPrefix "H" "Hrs_".
+      wp_apply (controller.wp_GetPodFromTemplate_ReplicaSet with "[$Hrs_HTemplate $Hrs_Hdeepown_template
+        $Hdeepown_m_l_rs $Hdeepown_l_controller_ref]").
+      { destruct Hrs_valid as (Hrs_meta_valid & Hrs_spec_valid & _).
+        pose proof (ReplicaSetSpecV.valid_template _ Hrs_spec_valid) as Hrs_valid_template.
+        iPureIntro. split_and!. all: try done. }
+      iIntros (pod_l pod) "(Hdeepown_l_pod & %Hpr & %Hvalid & Hrs_HTemplate & Hrs_Hdeepown_template & Hdeepown_m_l_rs)".
+      wp_auto. rewrite bool_decide_true //. wp_auto.
+      wp_apply (v1.wp_GetNamespace_deepown with "[$Hdeepown_m_l_rs]") as "Hdeepown_m_l_rs".
+      wp_apply wp_globals_get.
+      wp_apply (wp_State__PodCreate_nameless with "[$Hdeepown_l_pod $Hown_children_frag]").
+      { iFrame "#". iSplit.
+        - iAssert (is_pkg_init code.controllers.common.common) as "H". all: iPkgInit.
+        - iPureIntro. split_and!. all: try done.
+          + destruct Hrs_valid as (Hrs_meta_valid & _).
+            unfold ObjectMetaV.valid in Hrs_meta_valid. naive_solver.
+          + destruct Hrs_valid as (Hrs_meta_valid & _).
+            unfold ObjectMetaV.valid in Hrs_meta_valid. naive_solver.
+      }
+      iIntros (pod_l' pod' key uid) "H". iNamedPrefix "H" "Hcreate_". subst key. subst uid. wp_auto.
+      rewrite bool_decide_true //. wp_auto.
+      iApply wp_for_post_do. wp_auto.
+      iAssert (I) with "[Hi_ptr Hown_pod_meta_frags Hcreate_Hown_meta Hcreate_Hown_children]" as "loop_inv".
+      { iExists (word.add i (W64 1)), (pods' ++ [pod']). iFrame "Hi_ptr".
+        iSplitL "Hown_pod_meta_frags Hcreate_Hown_meta".
+        - rewrite big_sepL_app. simpl. iFrame.
+        - iSplitL "Hcreate_Hown_children".
+          + assert (list_to_set (PodV.key <$> pods') ∪ {[PodV.key pod']} = list_to_set (PodV.key <$> pods' ++ [pod']))
+              as ->.
+            { rewrite fmap_app. set_solver. }
+            done.
+          + iPureIntro.
+            split_and!.
+            * rewrite Forall_app. split; [done|].
+              constructor; [|constructor].
+              unfold is_pod_alive.
+              unfold ObjectMetaV.nameless_created in Hcreate_Hmeta_created.
+              naive_solver.
+            * rewrite app_length /= Hlength_eq'.
+              word.
+            * word.
+            * word.
+      }
+      iFrame. iApply (struct_fields_combine (V:=v1.ReplicaSetSpec.t)). iFrame.
+    + iApply "HΦ". iFrame. iSplitR. 1: iPureIntro; word. iSplitR. 1: done.
+      iApply ReplicaSetV.deepown_l_restore. iFrame.
+      iSplitR. 1: done. iSplitL. 2: done.
+      rewrite Hreplicas_eq. iExists n. iSplitL. all: done.
+  - admit.
+Admitted.
+
+Lemma wp_syncReplicaSet γ l (gv: schema.GroupVersion.t) namespace name rs pods :
+  {{{ is_pkg_init code.controllers.replicaset.replicaset ∗
+      "#Hisk" ∷ is_kubernetes γ l ∗
+      "#Hglobal_l" ∷ (global_addr common.State) ↦□ l ∗
+      "#Hglobal_gv" ∷ (global_addr v1.SchemeGroupVersion) ↦□ gv ∗
+      "Hown_rs_meta_frag" ∷ own_meta_frag γ (ReplicaSetV.key rs) rs.(ReplicaSetV.ObjectMeta').(ObjectMetaV.UID') 1
+        rs.(ReplicaSetV.ObjectMeta') ∗
       "Hown_pod_meta_frags" ∷ ([∗ list] k ↦ pod ∈ pods,
         own_meta_frag γ (PodV.key pod) pod.(PodV.ObjectMeta').(ObjectMetaV.UID') 1 pod.(PodV.ObjectMeta')) ∗
-      "Hown_children_frag" ∷ own_children_frag γ (ReplicaSetV.key rs) uid 1 (list_to_set (PodV.key <$> pods)) ∗
+      "Hown_children_frag" ∷ own_children_frag γ (ReplicaSetV.key rs) rs.(ReplicaSetV.ObjectMeta').(ObjectMetaV.UID') 1
+        (list_to_set (PodV.key <$> pods)) ∗
       "%Hnamespace_eq" ∷ ⌜ namespace = rs.(ReplicaSetV.ObjectMeta').(ObjectMetaV.Namespace') ⌝ ∗
       "%Hname_eq" ∷ ⌜ name = rs.(ReplicaSetV.ObjectMeta').(ObjectMetaV.Name') ⌝ ∗
       "%Hdeletion_timestamp_eq" ∷ ⌜ rs.(ReplicaSetV.ObjectMeta').(ObjectMetaV.DeletionTimestamp') = None ⌝ ∗
@@ -36,10 +158,12 @@ Lemma wp_syncReplicaSet γ l (gv: schema.GroupVersion.t) namespace name uid rs p
     @! replicaset.syncReplicaSet #namespace #name
   {{{ (pods' : list PodV.t), RET #interface.nil;
       ⌜ current_state_matches rs pods' ⌝ ∗
-      own_meta_frag γ (ReplicaSetV.key rs) uid 1 rs.(ReplicaSetV.ObjectMeta') ∗
+      own_meta_frag γ (ReplicaSetV.key rs) rs.(ReplicaSetV.ObjectMeta').(ObjectMetaV.UID') 1
+        rs.(ReplicaSetV.ObjectMeta') ∗
       ([∗ list] pod ∈ pods',
         own_meta_frag γ (PodV.key pod) pod.(PodV.ObjectMeta').(ObjectMetaV.UID') 1 pod.(PodV.ObjectMeta')) ∗
-      own_children_frag γ (ReplicaSetV.key rs) uid 1 (list_to_set (PodV.key <$> pods'))
+      own_children_frag γ (ReplicaSetV.key rs) rs.(ReplicaSetV.ObjectMeta').(ObjectMetaV.UID') 1
+        (list_to_set (PodV.key <$> pods'))
   }}}.
 Proof. Admitted.
 
